PropositionalLogic/IntuitionisticPropositionalLogic.v
@@ -19,3 +19,164 @@ Class IntuitionisticPropositionalLogic (L: Language) {nL: NormalLanguage L} {pL:
   falsep_elim: forall x, |-- FF --> x
 }.
 
+Lemma andp_intros_derivable: forall {L: Language} {nL: NormalLanguage L} {pL: PropositionalLanguage L} {Gamma: ProofTheory L} {nGamma: NormalProofTheory L Gamma} {mpGamma: MinimunPropositionalLogic L Gamma} {ipGamma: IntuitionisticPropositionalLogic L Gamma} (Phi: context) (x y: expr),
+  Phi |-- x --> y --> x && y.
+Proof.
+  intros.
+  pose proof andp_intros x y.
+  rewrite provable_derivable in H.
+  eapply derivable_weaken; eauto.
+  intros ? [].
+Qed.
+
+Lemma andp_elim1_derivable: forall {L: Language} {nL: NormalLanguage L} {pL: PropositionalLanguage L} {Gamma: ProofTheory L} {nGamma: NormalProofTheory L Gamma} {mpGamma: MinimunPropositionalLogic L Gamma} {ipGamma: IntuitionisticPropositionalLogic L Gamma} (Phi: context) (x y: expr),
+  Phi |-- x && y --> x.
+Proof.
+  intros.
+  pose proof andp_elim1 x y.
+  rewrite provable_derivable in H.
+  eapply derivable_weaken; eauto.
+  intros ? [].
+Qed.
+
+Lemma andp_elim2_derivable: forall {L: Language} {nL: NormalLanguage L} {pL: PropositionalLanguage L} {Gamma: ProofTheory L} {nGamma: NormalProofTheory L Gamma} {mpGamma: MinimunPropositionalLogic L Gamma} {ipGamma: IntuitionisticPropositionalLogic L Gamma} (Phi: context) (x y: expr),
+  Phi |-- x && y --> y.
+Proof.
+  intros.
+  pose proof andp_elim2 x y.
+  rewrite provable_derivable in H.
+  eapply derivable_weaken; eauto.
+  intros ? [].
+Qed.
+
+Lemma orp_intros1_derivable: forall {L: Language} {nL: NormalLanguage L} {pL: PropositionalLanguage L} {Gamma: ProofTheory L} {nGamma: NormalProofTheory L Gamma} {mpGamma: MinimunPropositionalLogic L Gamma} {ipGamma: IntuitionisticPropositionalLogic L Gamma} (Phi: context) (x y: expr),
+  Phi |-- x --> x || y.
+Proof.
+  intros.
+  pose proof orp_intros1 x y.
+  rewrite provable_derivable in H.
+  eapply derivable_weaken; eauto.
+  intros ? [].
+Qed.
+
+Lemma orp_intros2_derivable: forall {L: Language} {nL: NormalLanguage L} {pL: PropositionalLanguage L} {Gamma: ProofTheory L} {nGamma: NormalProofTheory L Gamma} {mpGamma: MinimunPropositionalLogic L Gamma} {ipGamma: IntuitionisticPropositionalLogic L Gamma} (Phi: context) (x y: expr),
+  Phi |-- y --> x || y.
+Proof.
+  intros.
+  pose proof orp_intros2 x y.
+  rewrite provable_derivable in H.
+  eapply derivable_weaken; eauto.
+  intros ? [].
+Qed.
+
+Lemma orp_elim_derivable: forall {L: Language} {nL: NormalLanguage L} {pL: PropositionalLanguage L} {Gamma: ProofTheory L} {nGamma: NormalProofTheory L Gamma} {mpGamma: MinimunPropositionalLogic L Gamma} {ipGamma: IntuitionisticPropositionalLogic L Gamma} (Phi: context) (x y z: expr),
+  Phi |-- (x --> z) --> (y --> z) --> (x || y --> z).
+Proof.
+  intros.
+  pose proof orp_elim x y z.
+  rewrite provable_derivable in H.
+  eapply derivable_weaken; eauto.
+  intros ? [].
+Qed.
+
+Lemma falsep_elim_derivable: forall {L: Language} {nL: NormalLanguage L} {pL: PropositionalLanguage L} {Gamma: ProofTheory L} {nGamma: NormalProofTheory L Gamma} {mpGamma: MinimunPropositionalLogic L Gamma} {ipGamma: IntuitionisticPropositionalLogic L Gamma} (Phi: context) (x: expr),
+  Phi |-- FF --> x.
+Proof.
+  intros.
+  pose proof falsep_elim x.
+  rewrite provable_derivable in H.
+  eapply derivable_weaken; eauto.
+  intros ? [].
+Qed.
+
+Lemma DCS_andp_iff: forall {L: Language} {nL: NormalLanguage L} {pL: PropositionalLanguage L} {Gamma: ProofTheory L} {nGamma: NormalProofTheory L Gamma} {mpGamma: MinimunPropositionalLogic L Gamma} {ipGamma: IntuitionisticPropositionalLogic L Gamma} (Phi: context),
+  derivable_closed Phi ->
+  (forall x y: expr, Phi (x && y) <-> (Phi x /\ Phi y)).
+Proof.
+  intros.
+  pose proof derivable_closed_element_derivable _ H; clear H.
+  rewrite !H0; clear H0; split; intros.
+  + pose proof andp_elim1_derivable Phi x y.
+    pose proof andp_elim2_derivable Phi x y.
+    split; apply derivable_modus_ponens with (x && y); auto.
+  + pose proof andp_intros_derivable Phi x y.
+    destruct H.
+    apply derivable_modus_ponens with y; auto.
+    apply derivable_modus_ponens with x; auto.
+Qed.
+
+Lemma DCS_orp_iff: forall {L: Language} {nL: NormalLanguage L} {pL: PropositionalLanguage L} {Gamma: ProofTheory L} {nGamma: NormalProofTheory L Gamma} {mpGamma: MinimunPropositionalLogic L Gamma} {ipGamma: IntuitionisticPropositionalLogic L Gamma} (Phi: context),
+  derivable_closed Phi ->
+  orp_witnessed Phi ->
+  (forall x y: expr, Phi (x || y) <-> (Phi x \/ Phi y)).
+Proof.
+  intros.
+  pose proof derivable_closed_element_derivable _ H; clear H.
+  split; intros.
+  + apply H0; auto.
+  + rewrite !H1 in *.
+    destruct H.
+    - pose proof orp_intros1_derivable Phi x y.
+      apply derivable_modus_ponens with x; auto.
+    - pose proof orp_intros2_derivable Phi x y.
+      apply derivable_modus_ponens with y; auto.
+Qed.
+
+Lemma intuitionistic_reduction_consistent: forall {L: Language} {nL: NormalLanguage L} {pL: PropositionalLanguage L} {Gamma: ProofTheory L} {nGamma: NormalProofTheory L Gamma} {mpGamma: MinimunPropositionalLogic L Gamma} {ipGamma: IntuitionisticPropositionalLogic L Gamma}, reduction_consistent_prooftheory IntuitionisticReduction Gamma.
+Proof.
+  intros.
+  apply reduction_consistent_prooftheory_from_provable; auto.
+  hnf; intros.
+  apply syntactic_reduction_rule; auto.
+Qed.
+
+Module IntuitionisticPropositionalLogic.
+Section IntuitionisticPropositionalLogic.
+
+Context (Var: Type).
+
+Inductive provable: @expr (PropositionalLanguage.L Var) -> Prop :=
+| syntactic_reduction_rule1: forall x y, @reduce _ IntuitionisticReduction x y -> provable x -> provable y
+| syntactic_reduction_rule2: forall x y, @reduce _ IntuitionisticReduction x y -> provable y -> provable x
+| modus_ponens: forall x y, provable (x --> y) -> provable x -> provable y
+| axiom1: forall x y, provable (x --> (y --> x))
+| axiom2: forall x y z, provable ((x --> y --> z) --> (x --> y) --> (x --> z))
+| andp_intros: forall x y, provable (x --> y --> x && y)
+| andp_elim1: forall x y, provable (x && y --> x)
+| andp_elim2: forall x y, provable (x && y --> y)
+| orp_intros1: forall x y, provable (x --> x || y)
+| orp_intros2: forall x y, provable (y --> x || y)
+| orp_elim: forall x y z, provable ((x --> z) --> (y --> z) --> (x || y --> z))
+| falsep_elim: forall x, provable (FF --> x).
+
+Instance AG: AxiomaticProofTheory.AxiomaticProofTheory (PropositionalLanguage.L Var) :=
+  AxiomaticProofTheory.Build_AxiomaticProofTheory (PropositionalLanguage.L Var) provable.
+
+Instance G: ProofTheory (PropositionalLanguage.L Var) := AxiomaticProofTheory.G AG.
+
+Instance mpG: MinimunPropositionalLogic (PropositionalLanguage.L Var) G.
+Proof.
+  constructor.
+  + apply modus_ponens.
+  + apply axiom1.
+  + apply axiom2.
+Qed.
+
+Instance ipG: IntuitionisticPropositionalLogic (PropositionalLanguage.L Var) G.
+Proof.
+  constructor.
+  + split.
+    - apply syntactic_reduction_rule1; auto. 
+    - apply syntactic_reduction_rule2; auto. 
+  + apply andp_intros.
+  + apply andp_elim1.
+  + apply andp_elim2.
+  + apply orp_intros1.
+  + apply orp_intros2.
+  + apply orp_elim.
+  + apply falsep_elim.
+Qed.
+
+End IntuitionisticPropositionalLogic.
+End IntuitionisticPropositionalLogic.
+
