PropositionalLogic/Complete_Intuitionistic_Kripke.v
@@ -1,0 +1,227 @@
+Require Import Logic.lib.Bijection.
+Require Import Logic.lib.Countable.
+Require Import Logic.LogicBase.
+Require Import Logic.SyntacticReduction.
+Require Import Logic.HenkinCompleteness.
+Require Import Logic.PropositionalLogic.Syntax.
+Require Import Logic.PropositionalLogic.MinimunPropositionalLogic.
+Require Import Logic.PropositionalLogic.IntuitionisticPropositionalLogic.
+Require Import Logic.PropositionalLogic.KripkeSemantics.
+
+Local Open Scope logic_base.
+Local Open Scope PropositionalLogic.
+
+Definition DCS (Var: Type): Type := sig (fun Phi =>
+  @derivable_closed _ _ (IntuitionisticPropositionalLogic.G Var) Phi /\
+  @orp_witnessed _ _ _ (IntuitionisticPropositionalLogic.G Var) Phi /\
+  consistent (IntuitionisticPropositionalLogic.G Var) Phi).
+
+Definition canonical_frame (Var: Type): KripkeSemantics.frame.
+  refine (KripkeSemantics.Build_frame (DCS Var) (fun a b => Included _ (proj1_sig b) (proj1_sig a)) _).
+  constructor.
+  + hnf; intros.
+    hnf; intros; auto.
+  + hnf; intros.
+    hnf; intros; auto.
+Defined.
+
+Program Definition canonical_eval (Var: Type): Var -> KripkeSemantics.sem (canonical_frame Var) :=
+  fun p a => a (PropositionalLanguage.varp p).
+Next Obligation.
+  apply H; auto.
+Qed.
+
+Definition canonical_model {Var: Type} (Phi: DCS Var): @model _ (KripkeSemantics.SM Var) :=
+  KripkeSemantics.Build_model Var (canonical_frame Var) (canonical_eval Var) Phi.
+
+Lemma Lindenbaum_lemma {Var: Type}: Countable Var ->
+  forall Phi x,
+    ~ @derivable _ (IntuitionisticPropositionalLogic.G Var) Phi x ->
+    exists Psi,
+      Included _ Phi Psi /\
+      ~ @derivable _ (IntuitionisticPropositionalLogic.G Var) Psi x /\
+      @derivable_closed _ _ (IntuitionisticPropositionalLogic.G Var) Psi /\
+      @orp_witnessed _ _ _ (IntuitionisticPropositionalLogic.G Var) Psi /\
+      consistent (IntuitionisticPropositionalLogic.G Var) Psi.
+Proof.
+  intros.
+  apply PropositionalLanguage.formula_countable in X.
+  set (step :=
+          fun n Phi x0 =>
+             Phi x0 \/
+            (inj_R _ _ X x0 n /\
+             ~ @derivable _ (IntuitionisticPropositionalLogic.G Var) (Union _ Phi (Singleton _ x0)) x)).
+  exists (LindenbaumConstruction step Phi).
+  assert (Included expr Phi (LindenbaumConstruction step Phi) /\
+          ~ @derivable _ (IntuitionisticPropositionalLogic.G Var) (LindenbaumConstruction step Phi) x /\
+          (~ @derivable _ (IntuitionisticPropositionalLogic.G Var) (LindenbaumConstruction step Phi) x ->
+           @derivable_closed _ _ (IntuitionisticPropositionalLogic.G Var) (LindenbaumConstruction step Phi)) /\
+          (~ @derivable _ (IntuitionisticPropositionalLogic.G Var) (LindenbaumConstruction step Phi) x ->
+           @orp_witnessed _ _ _ (IntuitionisticPropositionalLogic.G Var) (LindenbaumConstruction step Phi))).
+  Focus 2. {
+    destruct H0 as [? [? [? ?]]].
+    split; [| split; [| split; [| split]]]; auto.
+    intro; apply H1.
+    pose proof @falsep_elim_derivable _ _ _ _ _ _ (IntuitionisticPropositionalLogic.ipG Var) (LindenbaumConstruction step Phi) x.
+    eapply (@derivable_modus_ponens _ _ _ _ _ (IntuitionisticPropositionalLogic.mpG Var) (LindenbaumConstruction step Phi)); [exact H4 | exact H5].
+  } Unfocus.
+  split; [| split; [| split]].
+  + apply (Lindenbaum_spec_included _ _ 0).
+  + apply (Lindenbaum_spec_pos _ _
+            (fun xs => @provable _ (IntuitionisticPropositionalLogic.G Var) (multi_imp xs x))
+            (fun Phi => @derivable _ (IntuitionisticPropositionalLogic.G Var) Phi x)).
+    - intros; apply derivable_provable.
+    - intros ? ? ? ?; left; auto.
+    - apply H.
+    - intros.
+      destruct (Classical_Prop.classic (exists x0, inj_R _ _ X x0 n /\ ~ @derivable _ (IntuitionisticPropositionalLogic.G Var) (Union _ S (Singleton _ x0)) x)) as [[x0 [? ?]] |].
+      * intro; apply H2; clear H2.
+        eapply derivable_weaken; [| exact H3].
+        hnf; intros ? [? | [? ?]]; [left; auto |].
+        pose proof in_inj _ _ X _ _ _ H1 H2.
+        subst; right; constructor.
+      * intro; apply H0; clear H0.
+        eapply derivable_weaken; [| exact H2].
+        hnf; intros ? [? | [? ?]]; [auto |].
+        exfalso; apply H1; clear H1.
+        exists x0; auto.
+  + intros; hnf; intros.
+    destruct (im_inj _ _ X x0) as [n ?].
+    apply (Lindenbaum_spec_neg _ _ _ (S n)).
+    simpl.
+    unfold step at 1.
+    right; split; auto.
+    intro.
+    rewrite (@deduction_theorem _ _ _ _ _ (IntuitionisticPropositionalLogic.mpG Var)) in H3.
+    eapply derivable_weaken in H3; [| apply (Lindenbaum_spec_included _ _ n)].
+    pose proof @derivable_modus_ponens _ _ _ _ _ (IntuitionisticPropositionalLogic.mpG Var) _ _ _ H1 H3.
+    auto.
+  + intros; hnf; intros x0 y0 ?.
+    destruct (im_inj _ _ X x0) as [nx ?].
+    destruct (im_inj _ _ X y0) as [ny ?].
+    assert (LindenbaumChain step Phi (S nx) x0 \/ LindenbaumChain step Phi (S ny) y0) as HH;
+      [| destruct HH as [HH | HH]; apply Lindenbaum_spec_neg in HH; auto].
+    simpl.
+    unfold step at 1 3.
+    assert (~ @derivable _ (IntuitionisticPropositionalLogic.G Var) (Union _ (LindenbaumChain step Phi nx) (Singleton _ x0)) x \/ ~ @derivable _ (IntuitionisticPropositionalLogic.G Var) (Union _ (LindenbaumChain step Phi ny) (Singleton _ y0)) x) as HH;
+      [| destruct HH as [HH | HH]; auto].
+    apply Classical_Prop.not_and_or; intros [? ?].
+    rewrite (@deduction_theorem _ _ _ _ _ (IntuitionisticPropositionalLogic.mpG Var)) in H4, H5.
+    eapply derivable_weaken in H4; [| apply (Lindenbaum_spec_included _ _ nx)].
+    eapply derivable_weaken in H5; [| apply (Lindenbaum_spec_included _ _ ny)].
+    pose proof @orp_elim_derivable _ _ _ _ _ _ (IntuitionisticPropositionalLogic.ipG Var) (LindenbaumConstruction step Phi) x0 y0 x.
+    pose proof @derivable_modus_ponens _ _ _ _ _ (IntuitionisticPropositionalLogic.mpG Var) _ _ _ H4 H6.
+    pose proof @derivable_modus_ponens _ _ _ _ _ (IntuitionisticPropositionalLogic.mpG Var) _ _ _ H5 H7.
+    apply (@derivable_assum _ _ _ _ _ (IntuitionisticPropositionalLogic.mpG Var) _ (x0 || y0)) in H1.
+    pose proof @derivable_modus_ponens _ _ _ _ _ (IntuitionisticPropositionalLogic.mpG Var) _ _ _ H1 H8.
+    auto.
+Qed.
+
+Lemma truth_lemma {Var: Type} {CV: Countable Var}: forall (Phi: DCS Var) x, canonical_model Phi |= x <-> proj1_sig Phi x.
+Proof.
+  intros.
+  revert x.
+  pose proof (fun Phi: DCS Var => @derivable_closed_element_derivable _ _ _ _ _ (IntuitionisticPropositionalLogic.mpG Var) (proj1_sig Phi) (proj1 (proj2_sig Phi))).
+  pose proof @KripkeSemantics.intuitionistic_consistent Var.
+  pose proof @intuitionistic_reduction_consistent _ _ _ _  _ _ (IntuitionisticPropositionalLogic.ipG Var).
+  apply (@truth_lemma_from_syntactic_reduction  _ _ (PropositionalLanguage.nIntuitionisticReduction) _ _ H1 H0 _ _ (H Phi)).
+  intros.
+  clear H0 H1.
+  revert Phi.
+  induction x; try solve [inversion H2]; intros.
+  + destruct H2.
+    specialize (IHx1 H0 Phi).
+    specialize (IHx2 H1 Phi).
+    pose proof @DCS_andp_iff _ _ _ _ _ _ (IntuitionisticPropositionalLogic.ipG Var) (proj1_sig Phi) (proj1 (proj2_sig Phi)) x1 x2.
+    simpl in *.
+    unfold KripkeSemantics.sem_and.
+    tauto.
+  + destruct H2.
+    specialize (IHx1 H0 Phi).
+    specialize (IHx2 H1 Phi).
+    pose proof @DCS_orp_iff _ _ _ _ _ _ (IntuitionisticPropositionalLogic.ipG Var) (proj1_sig Phi) (proj1 (proj2_sig Phi)) (proj1 (proj2 (proj2_sig Phi))) x1 x2.
+    simpl in *.
+    unfold KripkeSemantics.sem_or.
+    tauto.
+  + destruct H2.
+    specialize (IHx1 H0).
+    specialize (IHx2 H1).
+    split.
+    - intros.
+      rewrite H.
+      apply (@deduction_theorem _ _ _ _ _ (IntuitionisticPropositionalLogic.mpG Var)).
+      apply Classical_Prop.NNPP; intro.
+      pose proof Lindenbaum_lemma CV _ _ H3.
+      destruct H4 as [Psi [? [? ?]]].
+      hnf in H2.
+      specialize (H2 (exist _ Psi H6)).
+      assert (Included _ (proj1_sig Phi) Psi) by (hnf; intros; apply H4; left; auto).
+      specialize (H2 H7).
+      simpl in IHx1, IHx2.
+      change (KripkeSemantics.model_frame (canonical_model Phi)) with (canonical_frame Var) in H2.
+      change (KripkeSemantics.model_var (canonical_model Phi)) with (canonical_eval Var) in H2.
+      rewrite IHx1, IHx2 in H2; simpl in H2.
+      assert (Psi x1) by (apply H4; right; constructor).
+      specialize (H2 H8).
+      specialize (H (exist _ Psi H6) x2); simpl in H.
+      rewrite H in H2; auto.
+    - intros.
+      hnf; intros Psi ?H.
+      change (DCS Var) in Psi.
+      simpl in H3.
+      change (KripkeSemantics.model_frame (canonical_model Phi)) with (canonical_frame Var).
+      change (KripkeSemantics.model_var (canonical_model Phi)) with (canonical_eval Var).
+      simpl in IHx1, IHx2.
+      rewrite IHx1, IHx2.
+      intros.
+      rewrite H in H2, H4 |- *.
+      eapply derivable_weaken in H2; [| exact H3].
+      exact (@derivable_modus_ponens _ _ _ _ _ (IntuitionisticPropositionalLogic.mpG Var) _ _ _ H4 H2).
+  + simpl.
+    split; [intros [] | intros].
+    rewrite H in H0.
+    pose proof proj2_sig Phi.
+    destruct H1 as [_ [_ ?]].
+    apply H1; auto.
+  + simpl.
+    unfold canonical_model.
+    tauto.
+Qed.
+
+Theorem complete_intuitionistic_kripke (Var: Type) (CV: Countable Var): strongly_complete (IntuitionisticPropositionalLogic.G Var) (KripkeSemantics.SM Var).
+Abort.
+(*
+Proof.
+  assert (forall Phi x, consistent (ClassicalPropositionalLogic.G Var) Phi -> satisfiable Phi).
+  + intros.
+    assert (exists Psi, Included _ Phi Psi /\ maximal_consistent (ClassicalPropositionalLogic.G Var) Psi)
+      by (apply Lindenbaum_lemma; auto).
+    destruct H0 as [Psi [? ?]].
+    exists (canonical_model (exist _ Psi H1)).
+    intros.
+    apply truth_lemma.
+    simpl.
+    apply H0; auto.
+  + hnf; intros.
+    specialize (H (Union _ Phi (Singleton _ (~~ x)))).
+    unfold consistent in H.
+    apply Classical_Prop.NNPP.
+    intro.
+    assert (satisfiable (Union expr Phi (Singleton expr (~~ x)))).
+    Focus 1. {
+      apply H.
+      intro; apply H1.
+      rewrite (@deduction_theorem _ _ _ _ _ (ClassicalPropositionalLogic.mpG Var)) in H2.
+      clear - H2.
+      apply (@aux_classic_theorem05 _ _ _ _ _ _ (ClassicalPropositionalLogic.cpG Var)); auto.
+    } Unfocus.
+    destruct H2 as [m ?].
+    specialize (H0 m).
+    pose proof (H2 (~~ x) (Union_intror _ _ _ _ (In_singleton _ _))).
+    pose proof (fun x H => H2 x (Union_introl _ _ _ _ H)).
+    specialize (H0 H4).
+    clear - H0 H3.
+    simpl in *; auto.
+Qed.
+
+*)
